src/Init/Data/Nat/Lemmas.lean
@@ -355,8 +355,8 @@ protected theorem sub_le_sub_iff_left {n m k : Nat} (h : n ≤ k) : k - m ≤ k 
 
 protected theorem sub_lt_of_pos_le (h₀ : 0 < a) (h₁ : a ≤ b) : b - a < b :=
   Nat.sub_lt (Nat.lt_of_lt_of_le h₀ h₁) h₀
-set_option linter.defProp false in
-protected abbrev sub_lt_self := @Nat.sub_lt_of_pos_le
+
+protected theorem sub_lt_self {a b : Nat} (h₁ : 0 < a) (h₂ : a ≤ b) : b - a < b := Nat.sub_lt_of_pos_le h₁ h₂
 
 theorem add_lt_of_lt_sub' {a b c : Nat} : b < c - a → a + b < c := by
   rw [Nat.add_comm]; exact Nat.add_lt_of_lt_sub
