src/Std/Data/Iterators/Lemmas/Producers/Range.lean
@@ -51,9 +51,6 @@ set_option linter.defProp false in
 @[deprecated Rcc.length_iter (since := "2026-01-28")]
 def Rcc.count_iter := @Rcc.length_iter
 
-set_option linter.defProp false in
-@[deprecated Rcc.length_iter (since := "2025-11-13")]
-def Rcc.count_iter_eq_size := @Rcc.length_iter
 
 @[simp]
 theorem Rco.toList_iter [LT α] [DecidableLT α] [UpwardEnumerable α]
@@ -91,10 +88,6 @@ set_option linter.defProp false in
 @[deprecated Rco.length_iter (since := "2026-01-28")]
 def Rco.count_iter := @Rco.length_iter
 
-set_option linter.defProp false in
-@[deprecated Rco.length_iter (since := "2025-11-13")]
-def Rco.count_iter_eq_size := @Rco.length_iter
-
 @[simp]
 theorem Rci.toList_iter [UpwardEnumerable α]
     [Rxi.IsAlwaysFinite α] [LawfulUpwardEnumerable α] {r : Rci α} :
@@ -130,10 +123,6 @@ theorem Rci.length_iter [UpwardEnumerable α]
 set_option linter.defProp false in
 @[deprecated Rci.length_iter (since := "2026-01-28")]
 def Rci.count_iter := @Rci.length_iter
-
-set_option linter.defProp false in
-@[deprecated Rci.length_iter (since := "2025-11-13")]
-def Rci.count_iter_eq_size := @Rci.length_iter
 
 @[simp]
 theorem Roc.toList_iter [LE α] [DecidableLE α] [UpwardEnumerable α]
@@ -171,10 +160,6 @@ set_option linter.defProp false in
 @[deprecated Roc.length_iter (since := "2026-01-28")]
 def Roc.count_iter := @Roc.length_iter
 
-set_option linter.defProp false in
-@[deprecated Roc.length_iter (since := "2025-11-13")]
-def Roc.count_iter_eq_size := @Roc.length_iter
-
 @[simp]
 theorem Roo.toList_iter [LT α] [DecidableLT α] [UpwardEnumerable α]
     [LawfulUpwardEnumerableLT α] [Rxo.IsAlwaysFinite α] [LawfulUpwardEnumerable α] {r : Roo α} :
@@ -210,10 +195,6 @@ theorem Roo.length_iter [LT α] [DecidableLT α] [UpwardEnumerable α]
 set_option linter.defProp false in
 @[deprecated Roo.length_iter (since := "2026-01-28")]
 def Roo.count_iter := @Roo.length_iter
-
-set_option linter.defProp false in
-@[deprecated Roo.length_iter (since := "2025-11-13")]
-def Roo.count_iter_eq_size := @Roo.length_iter
 
 @[simp]
 theorem Roi.toList_iter [UpwardEnumerable α]
@@ -251,10 +232,6 @@ set_option linter.defProp false in
 @[deprecated Roi.length_iter (since := "2026-01-28")]
 def Roi.count_iter := @Roi.length_iter
 
-set_option linter.defProp false in
-@[deprecated Roi.length_iter (since := "2025-11-13")]
-def Roi.count_iter_eq_size := @Roi.length_iter
-
 @[simp]
 theorem Ric.toList_iter [Least? α] [LE α] [DecidableLE α] [UpwardEnumerable α]
     [LawfulUpwardEnumerableLE α] [Rxc.IsAlwaysFinite α] [LawfulUpwardEnumerable α] {r : Ric α} :
@@ -290,10 +267,6 @@ theorem Ric.length_iter [Least? α] [LE α] [DecidableLE α] [UpwardEnumerable �
 set_option linter.defProp false in
 @[deprecated Ric.length_iter (since := "2026-01-28")]
 def Ric.count_iter := @Ric.length_iter
-
-set_option linter.defProp false in
-@[deprecated Ric.length_iter (since := "2025-11-13")]
-def Ric.count_iter_eq_size := @Ric.length_iter
 
 @[simp]
 theorem Rio.toList_iter [Least? α] [LT α] [DecidableLT α] [UpwardEnumerable α]
@@ -331,10 +304,6 @@ set_option linter.defProp false in
 @[deprecated Rio.length_iter (since := "2026-01-28")]
 def Rio.count_iter := @Rio.length_iter
 
-set_option linter.defProp false in
-@[deprecated Rio.length_iter (since := "2025-11-13")]
-def Rio.count_iter_eq_size := @Rio.length_iter
-
 @[simp]
 theorem Rii.toList_iter [Least? α] [UpwardEnumerable α]
     [Rxi.IsAlwaysFinite α] [LawfulUpwardEnumerable α] {r : Rii α} :
@@ -370,9 +339,5 @@ theorem Rii.length_iter [Least? α] [UpwardEnumerable α]
 set_option linter.defProp false in
 @[deprecated Rii.length_iter (since := "2026-01-28")]
 def Rii.count_iter := @Rii.length_iter
-
-set_option linter.defProp false in
-@[deprecated Rii.length_iter (since := "2025-11-13")]
-def Rii.count_iter_eq_size := @Rii.length_iter
 
 end Std
